\documentclass[12pt]{scrartcl}

\input{amslambda}

\usepackage{MnSymbol}

\newcommand{\leqg}{{\lambda{\simeq}_2}}

\newcommand{\unitt}{{\boldsymbol{1}}}
%\newcommand{\ttt}{\mathtt{t\!t}}
\newcommand{\idof}[1]{\mathsf{Id}{(#1)}}

\newcommand{\props}{\mathsf{Prop}}
\newcommand{\sets}{\mathsf{Set}}
\newcommand{\grpds}{\mathsf{Grpd}}
\newcommand{\TLRA}{\Lleftarrow\!\!\!\!\!\Rrightarrow}
\newcommand{\gequiv}{\TLRA}
\begin{document}
\pagestyle{empty}
\thispagestyle{empty}
\section*{\fbox{$\boldsymbol{\leqg}$}}
\subsubsection*{Syntax}
\begin{align*}
  t, A \quad ::= \quad \unitt &\mid \props \mid \sets \mid \grpds \mid
  \sta_3\\
&\mid P \lra Q \mid A \LRA B \mid G \gequiv H \mid (\Pi x {:} A) B \mid (\Sigma x {:} A) B \\
&\mid x \mid \ttt \mid \lambda x {:}A.t \mid s t \mid (s,t) \mid \pi_1 t \mid \pi_2 t \\
&\mid ({\sim}e) \mid e^+(t) \mid e^-(t) \mid \refl{t}\\
&\mid \sta^{\sta} \mid \Pi^* [x,x',x^*] {:} A^*. B^*
\mid \Sigma^* [x,x',x^*] {:} A^*. B^*
\mid {\ee{}^*} A^* B^*
\end{align*}
\subsubsection*{Typing}
The rules which appear below make use of the following
abbreviations.
\begin{align*}
\sta_2 &\df \grpds &
A \simeq_2 B &\df A \gequiv B \\
\sta_1 &\df \sets &
A \simeq_1 B &\df A  \LRA B\\
\sta_0 &\df \props &
A \simeq_0 B &\df A \lra B\\
\sta_{-1} &\df \unitt &
\idof{A} &\df \refl{A}\\
 a \sim_e b &\df ({\sim} e) a b&
a \ee A a' &\df a \sim_{\idof{A}} a'\\
\end{align*}

\begin{prooftree}
  \AXC{$k \in \setof{0,1,2,3}$}
  \UIC{$ \Gamma \vdash \sta_{k-1} : \sta_k$}
\end{prooftree}

\begin{prooftree}
  \AXC{$\Gamma \vdash A : \sta_k$}
  \AXC{$\Gamma, x : A \vdash B : \sta_k$}
\AXC{$ k \in \setof{0,1,2}$}
  \TIC{$\Gamma \vdash \Pi x{:}A.B : \sta_k$}
\end{prooftree}
\begin{prooftree}
  \AXC{$\Gamma \vdash A : \sta_k$}
  \AXC{$\Gamma, x : A \vdash B : \sta_k$}
\AXC{$ k \in \setof{0,1,2}$}
  \TIC{$\Gamma \vdash \Sigma x{:}A.B : \sta_k$}
\end{prooftree}
\begin{prooftree}
\AXC{$\Gamma \vdash A : \sta_k$}
\AXC{$\Gamma \vdash B : \sta_k$}
\AXC{$ k \in \setof{0,1,2}$}
\TIC{$\Gamma \vdash A \eeq_k B : \sta_k$}
\end{prooftree}
\begin{prooftree}
\AXC{$\Gamma \vdash A : \sta_k$\qquad$\Gamma \vdash B : \sta_k$}
\AXC{$\Gamma \vdash e : A \eeq_k B$}
\AXC{$k \in \setof{0,1,2}$}
\TIC{$\Gamma \vdash \;\,\sim_e\, : A \to B \to \sta_{k-1}$}
\end{prooftree}
\begin{prooftree}
\AXC{$e : A \eeq_k B$}
\AXC{$k \in \setof{0,1,2}$}
\BIC{$e^+ : A \to B$}
\noLine
\UIC{$e^- : B \to A$}
\end{prooftree}
\begin{prooftree}
  \AXC{$\Gamma \vdash A : \sta_k$}
  \AXC{$\Gamma \vdash a : A$}
  \AXC{$\Gamma \vdash k \in \setof{0,1,2}$}
  \TIC{$\Gamma \vdash \refl{a} : a \ee A a$}
\end{prooftree}


\newpage
\begin{prooftree}
  \AXC{$\Gamma \vdash A : \sta_k$}
  \AXC{$k \in \setof{0,1,2,3}$}
  \BIC{$\Gamma, x:A \vdash x:A$}
  \end{prooftree}
  \begin{prooftree}
  \AXC{$\Gamma \vdash M : A$}
  \AXC{$\Gamma \vdash B : \sta_k$}
  \AXC{$k \in \setof{0,1,2,3}$}
  \TIC{$\Gamma, y:B \vdash M:A$}
\end{prooftree}
\begin{prooftree}
  \AXC{$\Gamma \vdash A : *_k \qquad \Gamma \vdash B : *_k$}
  \AXC{$\Gamma \vdash M : A $}
  \AXC{$A = B \qquad k \in \setof{0,1,2}$}
  \TIC{$\Gamma \vdash M : B$}
\end{prooftree}
\vspace{1cm}

\begin{prooftree}
\AXC{}
\UIC{$\Gamma \vdash \ttt : \unitt$}
\end{prooftree}
\begin{prooftree}
    \AXC{$\Gamma \vdash A : *$}
    \AXC{$\Gamma, x : A \vdash B : *$}
    \AXC{$\Gamma, x : A \vdash b : B$}
    \TIC{$\Gamma \vdash \lambda x{:}A.b : \Pi x{:}A. B$}
  \end{prooftree}
  \begin{prooftree}
    \AXC{$\Gamma \vdash A : *\quad \Gamma, x: A \vdash B : *$}
    \AXC{$\Gamma \vdash f : \Pi x{:}A.B$}
    \AXC{$\Gamma \vdash a : A$}
    \TIC{$\Gamma \vdash f a : B[a/x]$}
  \end{prooftree}
\begin{prooftree}
  \AXC{$\Gamma \vdash A : * \quad \Gamma, x:A \vdash B : *$}
  \AXC{$\Gamma \vdash a : A$}
  \AXC{$\Gamma \vdash b : B[a/x]$}
  \TIC{$\Gamma \vdash (a,b) : \Sigma x{:}A.B$}
\end{prooftree}
  \begin{prooftree}
    \AXC{$\Gamma \vdash A : \sta$}
    \AXC{$\Gamma, x:A \vdash B : \sta$}
    \AXC{$\Gamma \vdash p : \Sigma x{:}A.B$}
    \TIC{$\begin{aligned}
        \Gamma &\vdash \pi_1 p : A\\
        \Gamma &\vdash \pi_2 p : B[\pi_1 p / x]
      \end{aligned}$}
    \end{prooftree}

\vspace{1cm}

\[
  \AXC{$\Gamma, x{:}A \vdash t : B$}
  \AXC{$\Gamma \vdash a : A$}
  \BIC{$\Gamma \vdash t[a /x] : B[a/x]$} 
  \DisplayProof
\qquad
  \AXC{$\Gamma, x{:}A \vdash t : B$}
  \AXC{$\Gamma \vdash a^* : a \ee A a'$}
  \BIC{$\Gamma \vdash t[a^* //x] : t[a/x] \sim_{B[a^*//x]} t[a'/x]$}
  \DisplayProof
\]

\[  \AXC{$\Gamma, \Delta \vdash t : B$}
  \AXC{$[\vec a/\vec x] \vdash \Gamma \RA \Delta$}
  \BIC{$\Gamma \vdash t[\vec a/ \vec x] : B[\vec a/
    \vec x]$} 
  \DisplayProof
\qquad
  \AXC{$\Gamma, \Delta \vdash t : B$}
  \AXC{$[\vec a^*//\vec x] : [\vec a/\vec x] \simeq [\vec a'/\vec x]
    \vdash \Gamma \RA \Delta$}
  \BIC{$\Gamma \vdash t[\vec a^*//\vec x] : t[\vec a/\vec x]
    \sim_{B[\vec a^*//\vec x]}  t[\vec a'/\vec x]$}
\DisplayProof
\]
\newcommand{\esub}{\between}
\newcommand{\esubs}{{\between}{\!}^*}
\[
\AXC{\phantom{$\Delta[\vec a / \vec x]$}}
\UIC{$\esub \vdash \Gamma \to \emptyset$}
\DisplayProof
\qquad
\AXC{$[\vec a/\vec x] \vdash \Gamma \RA \Delta$}
\AXC{$\Gamma, \Delta[\vec a/\vec x] \vdash   b[\vec a/\vec x] :
  B[\vec a/\vec x]$}
\BIC{$[\vec a, b / \vec x, y] \vdash \Gamma \RA \Delta, y:B$}
\DisplayProof
\]
\[
\AXC{\phantom{$\Delta[\vec a / \vec x]$}}
\UIC{$\esubs :\esub \simeq \esub \vdash \Gamma \to \emptyset$}
\DisplayProof
\qquad
\AXC{$\Bigg\{\begin{aligned}[]
[\vec a, b/\vec x,y] &\vdash \Gamma \RA \Delta, y:B \\
[\vec a', b'/\vec x,y] &\vdash \Gamma \RA \Delta, y:B
\end{aligned} \Bigg\}
$}
\noLine
\UIC{$[\vec a^*//\vec x] : [\vec a/\vec x] \simeq [\vec a'/\vec x]
: \Gamma \RA \Delta$}
\noLine
\UIC{$\Gamma, \Delta[\vec a^*//\vec x] \vdash   b^* :
  b \simeq_{B[\vec a^*//\vec x]} b'$}
\UIC{$[\vec a^*, b^* // \vec x, y] : [\vec a/\vec x] \simeq [\vec
  a'/\vec x] \vdash \Gamma \RA \Delta, y:B$}
\DisplayProof
\]
\end{document}

\begin{prooftree}
\AXC{$$}
\UIC{$\Gamma \vdash \sta^* : \sta \ee{} \sta$}
\end{prooftree}
\begin{prooftree}
\AXC{$\left.\begin{cases}
\Gamma \vdash A:*\\
\Gamma \vdash A':*\\
\Gamma \vdash A^* : A \ee{} A'
\end{cases}\right\}$}
\AXC{$\left.\begin{cases}
\phantom{x'{:}A',x^*{:}x {\sim_{A^*}} x'}\Gamma, x:A\;\: \vdash B:*\\
\phantom{x'{:}A',x^*{:}x {\sim_{A^*}} x'}\Gamma, x':A'\!\!\: \vdash B':*\\
\Gamma, x{:}A, x'{:}A', x^*:x {\sim_{A^*}} x' \vdash B^* : B \ee{} B'
\end{cases}\right\}$}
\BIC{$\Gamma \vdash \Pi^*[x,x',x^*]: A^*.\, B^* : \Pi x{:}A.B \ee{} \Pi x'{:}A'.B'$}
\noLine
\UIC{$\Gamma \vdash \Sigma^*[x,x',x^*]: A^*.\, B^* : \Sigma x{:}A.B \ee{} \Sigma x'{:}A'.B'$}
\end{prooftree}
\begin{prooftree}
  \AXC{$\left.\begin{cases}
\Gamma \vdash A:*\\
\Gamma \vdash A':*\\
\Gamma \vdash A^* : A \ee{} A'
\end{cases}\right\}$}
\AXC{$\left.\begin{cases}
\Gamma \vdash B:*\\
\Gamma \vdash B':*\\
\Gamma \vdash B^* : B \ee{} B'
\end{cases}\right\}$}
\BIC{$\Gamma \vdash \seq A^* B^* : (A \ee{} B) \ee{} (A' \ee{} B')$}
\end{prooftree}
